src/library/tactic/smt/smt_state.h
@@ -37,6 +37,7 @@ public:
     smt_goal(smt_config const & cfg);
     cc_state const & get_cc_state() const { return m_cc_state; }
     smt_pre_config const & get_pre_config() const { return m_pre_config; }
+    void add_lemma(hinst_lemma const & lemma) { m_em_state.add_lemma(lemma); }
 };
 
 class smt : public cc_propagation_handler {
