tests/lean/run/smt_ematch1.lean
@@ -8,3 +8,27 @@ begin [smt]
   trace_state,
   ematch
 end
+
+constant g : nat → nat → nat
+axiom gax : ∀ x, g x x = x
+
+example (a b c d e : nat) : d = a → c = e → g a d = b → b = g e c → f a = c :=
+begin [smt]
+  add_lemma gax,
+  ematch
+end
+
+local attribute [-ematch] fax
+
+example (a b c d e : nat) : d = a → c = e → g a d = b → b = g e c → f a = c :=
+begin [smt]
+  add_lemma [fax, gax],
+  ematch
+end
+
+example (a b c d e : nat) : (∀ x, g x (f x) = 0) → a = f b → g b a + 0 = f 0 :=
+begin [smt]
+   assert h : ∀ x, g x (f x) = 0,
+   add_lemma [h, fax, add_zero],
+   ematch
+end
